\begin{frame}
\frametitle{Derivation of project schemes, cont'd}
let 
\[
u^c = u^{n+1} - u^* 
\]
and 
\[
\phi =  (p^{n+1} - p^n) 
\]
then 
\begin{equation}
\label{eq1}
u^c - \frac{\Delta t}{\rho} \nabla \phi = 0 
\end{equation}
Further, since
\[
\nabla \cdot u^{n+1} = 0 
\]
we obtain 
\begin{equation}
\label{eq2}
\nabla \cdot u^c = - \nabla \cdot u^* 
\end{equation}
Inserting \eqref{eq1} into \eqref{eq2} we obtain
\[
- \frac{\Delta t}{\rho} \nabla^2 \phi = -\nabla \cdot u^*  
\]
We note that 
\[
u^{n+1} = u^* - u^c =  u^*- \frac{\Delta t}{\rho} \nabla \phi 
\]
\end{frame}

