\begin{frame}
  \frametitle{Solving the projection step}
  Applying $\nabla \cdot$ to 
  $
    \dfrac{u^{n+1} - u^{\bigstar}}{\Delta t} + \nabla p^{n+1} = 0
  $
  and using requirement $\nabla \cdot u^{n+1} = 0$ yields
  \begin{equation*}
    \Delta p^{n+1} = \dfrac{1}{\Delta t} \nabla  \cdot u^{\bigstar} \quad \text{in }
    \Omega
  \end{equation*}
  We already required
  \begin{equation*}
    p = 0 \quad \text{on } \partial \Omega_N
  \end{equation*}
  Multiplying 
  $
    \dfrac{u^{n+1} - u^{\bigstar}}{\Delta t} + \nabla p^{n+1} = 0
  $
  with $n$ and restricting to $\partial \Omega_D$ gives
  \begin{equation*}
    \dfrac{\partial p^{n+1}}{\partial n} = 0 \quad \text{on }
    \partial \Omega_D
  \end{equation*}
  Compute $u^{n+1}$ by
  \begin{equation*}
    u^{n+1} = u^{\bigstar} - \Delta t \nabla p^{n+1}
  \end{equation*}
  including boundary conditions for $u$ at $t = t^{n+1}$
\end{frame}

