\begin{frame}[fragile]
\frametitle{Code, cont'd}
\begin{python}
e0 = Constant((1, 0, 0))	
e1 = Constant((0, 1, 0))
e2 = Constant((0, 0, 1))
e3 = Expression(('-x[1]', 'x[0]', '0')) 
e4 = Expression(('-x[2]', '0', 'x[0]'))
e5 = Expression(('0', '-x[2]', 'x[1]'))
basis_vectors = [e0, e1, e2, e3, e4, e5]

a = 2*mu*inner(epsilon(u),epsilon(v))*dx + lambda_*inner(div(u),div(v))*dx

# Lagrange multipliers contrib to a
for i, e in enumerate(basis_vectors):
	r = rs[i]
	s = ss[i]
	a += r*inner(v, e)*dx + s*inner(u, e)*dx

\end{python}
\end{frame}
