\begin{frame}
  \frametitle{Semi-discrete system in space}
  Ansatz
  \begin{equation*}
    u_h(t) = \sum_{j=0}^N U_j(t) \phi_j
  \end{equation*}
Find $[U_1(t),\ldots, U_N(t)]^{\top}$
  \begin{equation*}
    \sum_{j=1}^N \dot U_j  (\phi_j,v_h)
    + \sum_{j=1}^N U_j a(\phi_j,v_h)
    = L(v_h)
  \end{equation*}
  or equivalently
%Find $[U_1(t),\ldots, U_N(t)]^{\top}$
  \begin{equation*}
    \sum_{j=1}^N \dot U_j  
    \underbrace{(\phi_j,\phi_i)}_{M_{ij}}
    + \sum_{j=1}^N U_j 
    \underbrace{a(\phi_j,\phi_i)}_{A_{ij}}
    = \underbrace{L(\phi_i)}_{b_i}
    \quad \foralls j = 1,\ldots,N
  \end{equation*}
  or equivalently
  \begin{equation*}
    M \dot U(t) + AU(t) = b(t)
  \end{equation*}
\end{frame}

